Deploying to gh-pages from @ xubaiw/reservoir-index@2f87a4a531528c3b3eaba917bfed674c50acc477 🚀

git/cruhland/lean4-axiomatic/Lean4Axiomatic/Natural.lean
@@ -1,6 +1,4 @@
 import Lean4Axiomatic.Natural.Exponentiation
-import Lean4Axiomatic.Natural.Order
-import Lean4Axiomatic.Natural.Sign
 
 namespace Lean4Axiomatic
 
@@ -18,34 +16,21 @@ required to construct an instance.
 **Named parameters**
 - `ℕ`: a type that obeys all of the properties provided by this class.
 -/
-class Natural (ℕ : Type) where
+class Natural (ℕ : Type) :=
   toCore : Core ℕ
   toAxioms : Axioms ℕ
   toAddition : Addition ℕ
   toSign : Sign ℕ
-  toOrder : Order.Derived ℕ
-  toMultiplication : Multiplication.Derived ℕ
-  toExponentiation : Exponentiation.Base ℕ
+  toOrder : Order ℕ
+  toMultiplication : Multiplication ℕ
+  toExponentiation : Exponentiation ℕ
 
-namespace Natural
+attribute [instance] Natural.toAddition
+attribute [instance] Natural.toAxioms
+attribute [instance] Natural.toCore
+attribute [instance] Natural.toExponentiation
+attribute [instance] Natural.toMultiplication
+attribute [instance] Natural.toOrder
+attribute [instance] Natural.toSign
 
-attribute [instance] toAddition
-attribute [instance] toAxioms
-attribute [instance] toCore
-attribute [instance] toMultiplication
-attribute [instance] toOrder
-attribute [instance] toSign
-
-export Exponentiation (powOp pow_step pow_zero)
-export Multiplication (
-  mul_associative mul_cancellative mul_commutative mul_distributive mulOp
-  mul_positive mul_split_zero mul_step mul_substitutive_eq mul_substitutive_lt
-  step_mul zero_mul
-)
-export Order (
-  le_antisymm le_defn le_reflexive le_split le_transitive leOp
-  lt_defn lt_defn_add ltOp lt_split lt_step lt_step_le lt_zero lt_zero_pos
-  trichotomy
-)
-
-end Lean4Axiomatic.Natural
+end Lean4Axiomatic
