git/cruhland/lean4-axiomatic/Lean4Axiomatic/Natural/Multiplication.lean
@@ -1,13 +1,15 @@
-import Lean4Axiomatic.Natural.Addition
 import Lean4Axiomatic.Natural.Order
-import Lean4Axiomatic.Natural.Sign
+
+/-!
+# Natural number multiplication
+-/
 
 namespace Lean4Axiomatic.Natural
 
 open Signed (Positive)
 
 /-!
-# Definition and properties of natural number multiplication
+## Axioms
 -/
 
 /--
@@ -15,7 +17,7 @@ Definition of multiplication, and properties that it must satisfy.
 
 All other properties of multiplication can be derived from these.
 -/
-class Multiplication.Base (ℕ : Type) [Core ℕ] [Addition ℕ] where
+class Multiplication (ℕ : Type) [Core ℕ] [Addition ℕ] :=
   /-- Definition of and syntax for multiplication. -/
   mulOp : Mul ℕ
 
@@ -28,73 +30,400 @@ class Multiplication.Base (ℕ : Type) [Core ℕ] [Addition ℕ] where
   -/
   step_mul {n m : ℕ} : step n * m ≃ (n * m) + m
 
-attribute [instance] Multiplication.Base.mulOp
+attribute [instance] Multiplication.mulOp
 
-/-- Properties that follow from those provided in `Multiplication.Base`. -/
-class Multiplication.Derived
-    (ℕ : Type) [Core ℕ] [Addition ℕ] [Sign ℕ] [Order.Base ℕ]
-    extends Multiplication.Base ℕ where
-  /--
-  Multiplication preserves equality of natural numbers; two equal natural
-  numbers are still equal after the same quantity is multiplied with both (on
-  the left or right).
-  -/
-  mul_substitutive_eq : AA.Substitutive₂ (α := ℕ) (· * ·) AA.tc (· ≃ ·) (· ≃ ·)
+export Multiplication (mulOp step_mul zero_mul)
 
-  /-- Multiplying by zero always gives zero. -/
-  mul_absorbing : AA.Absorbing (α := ℕ) 0 (· * ·)
+/-!
+## Derived properties
+-/
 
-  /--
-  Take a product and increment the right-hand factor. This gives the same
-  result as adding a copy of the left-hand factor to the original product.
-  -/
-  mul_step {n m : ℕ} : n * step m ≃ n * m + n
+variable {ℕ : Type}
+variable [Core ℕ]
+variable [Axioms ℕ]
+variable [Addition ℕ]
+variable [Sign ℕ]
+variable [Order ℕ]
+variable [Multiplication ℕ]
 
-  /-- The order of the factors in a product doesn't matter. -/
-  mul_commutative : AA.Commutative (α := ℕ) (· * ·)
+/--
+Multiplying by zero on the right always gives zero.
 
-  /-- A product is zero iff at least one of its factors is zero. -/
-  mul_split_zero {n m : ℕ} : n * m ≃ 0 ↔ n ≃ 0 ∨ m ≃ 0
+Intuition: the multiplication `count * value` is defined as `count` copies of
+`value` added together. So `n * 0` is `n` copies of `0` added together, which
+by properties of addition must always give `0`.
+-/
+theorem mul_zero {n : ℕ} : n * 0 ≃ 0 := by
+  apply ind_on (motive := λ x => x * 0 ≃ 0) n
+  case zero =>
+    show 0 * 0 ≃ 0
+    exact zero_mul
+  case step =>
+    intro n (ih : n * 0 ≃ 0)
+    show step n * 0 ≃ 0
+    calc
+      step n * 0 ≃ _ := step_mul
+      n * 0 + 0  ≃ _ := AA.substL ih
+      0 + 0      ≃ _ := Addition.zero_add
+      0          ≃ _ := Rel.refl
 
-  /-- The product of positive natural numbers is positive. -/
-  mul_positive {n m : ℕ} : Positive n → Positive m → Positive (n * m)
+instance mul_absorbing : AA.Absorbing (α := ℕ) 0 (· * ·) := {
+  absorbingL := AA.AbsorbingOn.mk zero_mul
+  absorbingR := AA.AbsorbingOn.mk mul_zero
+}
 
-  /--
-  Multiplication of a sum by a value is equivalent to summing the
-  multiplication of each term by that value.
-  -/
-  mul_distributive : AA.Distributive (α := ℕ) (· * ·) (· + ·)
+/--
+Take a product and increment the right-hand factor. This gives the same result
+as adding a copy of the left-hand factor to the original product.
 
-  /-- The grouping of the factors in a product doesn't matter. -/
-  mul_associative : AA.Associative (α := ℕ) (· * ·)
+This is a key lemma towards proving the commutativity of multiplication. Even
+though multiplication is defined as `count * value`, this result shows that it
+works just as well to swap the roles of `count` and `value`.
 
-  /-- Multiplication preserves strict order. -/
-  mul_substitutive_lt
+Intuition: `n` copies of `step m` added together can be rearranged into the sum
+of `n` copies of `m`, plus the sum of `n` copies of `1`. Since adding `n`
+copies of `1` together is just `n`, the whole result is `n * m + n`.
+-/
+theorem mul_step {n m : ℕ} : n * step m ≃ n * m + n := by
+  apply ind_on (motive := λ x => x * step m ≃ x * m + x) n
+  case zero =>
+    show 0 * step m ≃ 0 * m + 0
+    calc
+      0 * step m ≃ _ := zero_mul
+      0          ≃ _ := Rel.symm Addition.zero_add
+      0 + 0      ≃ _ := AA.substL (Rel.symm zero_mul)
+      0 * m + 0  ≃ _ := Rel.refl
+  case step =>
+    intro n (ih : n * step m ≃ n * m + n)
+    show step n * step m ≃ step n * m + step n
+    calc
+      step n * step m        ≃ _ := step_mul
+      n * step m + step m    ≃ _ := AA.substL ih
+      (n * m + n) + step m   ≃ _ := add_step
+      step ((n * m + n) + m) ≃ _ := AA.subst₁ AA.assoc
+      step (n * m + (n + m)) ≃ _ := AA.subst₁ (AA.substR AA.comm)
+      step (n * m + (m + n)) ≃ _ := AA.subst₁ (Rel.symm AA.assoc)
+      step ((n * m + m) + n) ≃ _ := AA.subst₁ (AA.substL (Rel.symm step_mul))
+      step (step n * m + n)  ≃ _ := Rel.symm add_step
+      step n * m + step n    ≃ _ := Rel.refl
+
+/--
+The order of the factors in a product doesn't matter.
+
+Intuition: combine the results from `mul_zero` and `mul_step`.
+-/
+theorem mul_comm {n m : ℕ} : n * m ≃ m * n := by
+  apply ind_on (motive := λ x => x * m ≃ m * x) n
+  case zero =>
+    show 0 * m ≃ m * 0
+    calc
+      0 * m ≃ _ := zero_mul
+      0     ≃ _ := Rel.symm mul_zero
+      m * 0 ≃ _ := Rel.refl
+  case step =>
+    intro n (ih : n * m ≃ m * n)
+    show step n * m ≃ m * step n
+    calc
+      step n * m ≃ _ := step_mul
+      n * m + m  ≃ _ := AA.substL ih
+      m * n + m  ≃ _ := Rel.symm mul_step
+      m * step n ≃ _ := Rel.refl
+
+instance mul_commutative : AA.Commutative (α := ℕ) (· * ·) := {
+  comm := mul_comm
+}
+
+/--
+Multiplication by a fixed value as the right-hand operand preserves equality.
+
+Intuition: addition preserves equality; multiplication is repeated addition.
+-/
+theorem subst_mul_eq {n₁ n₂ m : ℕ} : n₁ ≃ n₂ → n₁ * m ≃ n₂ * m := by
+  apply ind_on (motive := λ x => ∀ y, x ≃ y → x * m ≃ y * m) n₁
+  case zero =>
+    intro n₂
+    show 0 ≃ n₂ → 0 * m ≃ n₂ * m
+    apply cases_on (motive := λ y => 0 ≃ y → 0 * m ≃ y * m)
+    case zero =>
+      intro (_ : 0 ≃ (0 : ℕ))
+      show 0 * m ≃ 0 * m
+      exact Rel.refl
+    case step =>
+      intro n₂ (_ : 0 ≃ step n₂)
+      apply False.elim
+      show False
+      exact absurd (Rel.symm ‹0 ≃ step n₂›) Axioms.step_neq_zero
+  case step =>
+    intro n₁ (ih : ∀ y, n₁ ≃ y → n₁ * m ≃ y * m) n₂
+    show step n₁ ≃ n₂ → step n₁ * m ≃ n₂ * m
+    apply cases_on (motive := λ y => step n₁ ≃ y → step n₁ * m ≃ y * m)
+    case zero =>
+      intro (_ : step n₁ ≃ 0)
+      apply False.elim
+      show False
+      exact absurd ‹step n₁ ≃ 0› Axioms.step_neq_zero
+    case step =>
+      intro n₂ (_ : step n₁ ≃ step n₂)
+      show step n₁ * m ≃ step n₂ * m
+      have : n₁ ≃ n₂ := AA.inject ‹step n₁ ≃ step n₂›
+      have : n₁ * m ≃ n₂ * m := ih n₂ ‹n₁ ≃ n₂›
+      calc
+        step n₁ * m  ≃ _ := step_mul
+        (n₁ * m) + m ≃ _ := AA.substL ‹n₁ * m ≃ n₂ * m›
+        (n₂ * m) + m ≃ _ := Rel.symm step_mul
+        step n₂ * m  ≃ _ := Rel.refl
+
+def mul_substL_eq
+    : AA.SubstitutiveOn Hand.L (α := ℕ) (· * ·) AA.tc (· ≃ ·) (· ≃ ·)
+    := {
+  subst₂ := λ (_ : True) => subst_mul_eq
+}
+
+instance mul_substitutive_eq
+    : AA.Substitutive₂ (α := ℕ) (· * ·) AA.tc (· ≃ ·) (· ≃ ·)
+    := {
+  substitutiveL := mul_substL_eq
+  substitutiveR := AA.substR_from_substL_swap (rS := (· ≃ ·)) mul_substL_eq
+}
+
+/--
+A product is zero iff at least one of its factors is zero.
+
+Intuition
+- forwards: if one factor is nonzero, then the product is a nonempty sum that
+  results in zero. By `Addition.zero_sum_split`, the terms of the sum must be
+  zero.
+- backwards: by `Base.zero_mul` or `Derived.mul_zero`.
+-/
+theorem mul_split_zero {n m : ℕ} : n * m ≃ 0 ↔ n ≃ 0 ∨ m ≃ 0 := by
+  apply Iff.intro
+  · show n * m ≃ 0 → n ≃ 0 ∨ m ≃ 0
+    apply cases_on (motive := λ x => x * m ≃ 0 → x ≃ 0 ∨ m ≃ 0) n
+    case zero =>
+      intro (_ : 0 * m ≃ 0)
+      show 0 ≃ 0 ∨ m ≃ 0
+      exact Or.inl Rel.refl
+    case step =>
+      intro n (_ : step n * m ≃ 0)
+      show step n ≃ 0 ∨ m ≃ 0
+      apply Or.inr
+      show m ≃ 0
+      have : n * m + m ≃ 0 := calc
+        n * m + m  ≃ _ := Rel.symm step_mul
+        step n * m ≃ _ := ‹step n * m ≃ 0›
+        0          ≃ _ := Rel.refl
+      have ⟨_, (_ : m ≃ 0)⟩ := zero_sum_split ‹n * m + m ≃ 0›
+      exact ‹m ≃ 0›
+  · intro (_ : n ≃ 0 ∨ m ≃ 0)
+    show n * m ≃ 0
+    apply Or.elim ‹n ≃ 0 ∨ m ≃ 0›
+    · intro (_ : n ≃ 0)
+      show n * m ≃ 0
+      calc
+        n * m ≃ _ := AA.substL ‹n ≃ 0›
+        0 * m ≃ _ := zero_mul
+        0     ≃ _ := Rel.refl
+    · intro (_ : m ≃ 0)
+      show n * m ≃ 0
+      calc
+        n * m ≃ _ := AA.substR ‹m ≃ 0›
+        n * 0 ≃ _ := mul_zero
+        0     ≃ _ := Rel.refl
+
+/--
+The product of positive natural numbers is positive.
+
+Intuition: reframe positive as nonzero, then contradict with
+`Derived.mul_split_zero`.
+-/
+theorem mul_positive {n m : ℕ}
+    : Positive n → Positive m → Positive (n * m) := by
+  intro (_ : Positive n) (_ : Positive m)
+  show Positive (n * m)
+  have : n ≄ 0 := Signed.positive_defn.mp ‹Positive n›
+  have : m ≄ 0 := Signed.positive_defn.mp ‹Positive m›
+  apply Signed.positive_defn.mpr
+  show n * m ≄ 0
+  intro (_ : n * m ≃ 0)
+  show False
+  have : n ≃ 0 ∨ m ≃ 0 := mul_split_zero.mp ‹n * m ≃ 0›
+  apply Or.elim ‹n ≃ 0 ∨ m ≃ 0›
+  · intro (_ : n ≃ 0)
+    show False
+    exact absurd ‹n ≃ 0› ‹n ≄ 0›
+  · intro (_ : m ≃ 0)
+    show False
+    exact absurd ‹m ≃ 0› ‹m ≄ 0›
+
+/--
+Multiplication on the left distributes over addition.
+
+**Intuition**: Viewing `a * b` as the sum of `a` copies of `b`, this theorem
+says that the sum of `n` copies of `m + k` is the same as the sum of `n` copies
+of `m` added to the sum of `n` copies of `k`. Using the commutativity and
+associativity of addition to rearrange the sums shows this is clearly true.
+-/
+theorem mul_distribL_add {n m k : ℕ} : n * (m + k) ≃ n * m + n * k := by
+  apply ind_on (motive := λ x => x * (m + k) ≃ x * m + x * k) n
+  case zero =>
+    show 0 * (m + k) ≃ 0 * m + 0 * k
+    calc
+      0 * (m + k)   ≃ _ := zero_mul
+      0             ≃ _ := Rel.symm Addition.zero_add
+      0 + 0         ≃ _ := AA.substL (Rel.symm zero_mul)
+      0 * m + 0     ≃ _ := AA.substR (Rel.symm zero_mul)
+      0 * m + 0 * k ≃ _ := Rel.refl
+  case step =>
+    intro n (ih : n * (m + k) ≃ n * m + n * k)
+    show step n * (m + k) ≃ step n * m + step n * k
+    calc
+      step n * (m + k)          ≃ _ := step_mul
+      n * (m + k) + (m + k)     ≃ _ := AA.substL ih
+      n * m + n * k + (m + k)   ≃ _ := AA.assoc
+      n * m + (n * k + (m + k)) ≃ _ := AA.substR (Rel.symm AA.assoc)
+      n * m + ((n * k + m) + k) ≃ _ := AA.substR (AA.substL AA.comm)
+      n * m + ((m + n * k) + k) ≃ _ := AA.substR AA.assoc
+      n * m + (m + (n * k + k)) ≃ _ := Rel.symm AA.assoc
+      (n * m + m) + (n * k + k) ≃ _ := AA.substL (Rel.symm step_mul)
+      step n * m + (n * k + k)  ≃ _ := AA.substR (Rel.symm step_mul)
+      step n * m + step n * k   ≃ _ := Rel.refl
+
+def mul_distributiveL : AA.DistributiveOn Hand.L (α := ℕ) (· * ·) (· + ·) :=
+  AA.DistributiveOn.mk mul_distribL_add
+
+instance mul_distributive : AA.Distributive (α := ℕ) (· * ·) (· + ·) := {
+  distributiveL := mul_distributiveL
+  distributiveR := AA.distributiveR_from_distributiveL mul_distributiveL
+}
+
+/--
+The grouping of the factors in a product doesn't matter.
+
+**Intuition**: Imagine a collection of identical objects arranged into a
+rectangle `n * m` objects long and `k` objects high. Partition this into `m`
+smaller rectangles having length `n` and height `k`. Clearly the number of
+objects remains the same in both arrangements.
+-/
+instance mul_associative : AA.Associative (α := ℕ) (· * ·) := by
+  constructor
+  intro n m k
+  show (n * m) * k ≃ n * (m * k)
+  apply ind_on (motive := λ x => (x * m) * k ≃ x * (m * k))
+  case zero =>
+    show (0 * m) * k ≃ 0 * (m * k)
+    calc
+      (0 * m) * k ≃ _ := AA.substL zero_mul
+      0 * k       ≃ _ := zero_mul
+      0           ≃ _ := Rel.symm zero_mul
+      0 * (m * k) ≃ _ := Rel.refl
+  case step =>
+    intro n (ih : (n * m) * k ≃ n * (m * k))
+    show (step n * m) * k ≃ step n * (m * k)
+    calc
+      (step n * m) * k    ≃ _ := AA.substL step_mul
+      (n * m + m) * k     ≃ _ := AA.distribR
+      (n * m) * k + m * k ≃ _ := AA.substL ih
+      n * (m * k) + m * k ≃ _ := Rel.symm step_mul
+      step n * (m * k)    ≃ _ := Rel.refl
+
+/--
+Multiplication on the right by a positive natural number preserves the strict
+ordering of any two natural numbers.
+
+**Proof intuition**: two strictly ordered natural numbers have a positive
+difference between them. Multiplying them by another positive natural number
+also multiplies their difference, which remains positive.
+-/
+theorem subst_mul_lt
+    {n₁ n₂ m : ℕ} : Positive m → n₁ < n₂ → n₁ * m < n₂ * m := by
+  intro (_ : Positive m) (_ : n₁ < n₂)
+  show n₁ * m < n₂ * m
+  have ⟨(d : ℕ), (_ : Positive d), (_ : n₂ ≃ n₁ + d)⟩ :=
+    lt_defn_add.mp ‹n₁ < n₂›
+  have : n₂ * m ≃ n₁ * m + d * m := calc
+    n₂ * m         ≃ _ := AA.substL ‹n₂ ≃ n₁ + d›
+    (n₁ + d) * m   ≃ _ := AA.distribR
+    n₁ * m + d * m ≃ _ := Rel.refl
+  have : Positive (d * m) := mul_positive ‹Positive d› ‹Positive m›
+  exact lt_defn_add.mpr
+    ⟨d * m, ‹Positive (d * m)›, ‹n₂ * m ≃ n₁ * m + d * m›⟩
+
+def mul_substL_lt
+    : AA.SubstitutiveOn Hand.L (α := ℕ) (· * ·) Positive (· < ·) (· < ·)
+    := {
+  subst₂ := subst_mul_lt
+}
+
+instance mul_substitutive_lt
     : AA.Substitutive₂ (α := ℕ) (· * ·) Positive (· < ·) (· < ·)
+    := {
+  substitutiveL := mul_substL_lt
+  substitutiveR := AA.substR_from_substL_swap (rS := (· ≃ ·)) mul_substL_lt
+}
 
-  /--
-  A non-zero factor can be removed from products on both sides of an equality.
-  -/
-  mul_cancellative : AA.Cancellative (α := ℕ) (· * ·) (· ≄ 0) (· ≃ ·) (· ≃ ·)
+/--
+Multiplication on the left by a nonzero natural number is an injection.
 
-  /-- Multiplying a natural number by one produces the same natural number. -/
-  mul_identity : AA.Identity (α := ℕ) 1 (· * ·)
+**Proof intuition**: If one of the right-hand factors is greater than the other,
+then multiplying them both by a nonzero (i.e., positive) natural number will
+preserve their ordering (by `mul_substitutive_lt`), contradicting the hypothesis
+that the products are equal. Thus the right-hand factors must be equal.
+-/
+def mul_cancelL
+    : AA.CancellativeOn Hand.L (α := ℕ) (· * ·) (· ≄ 0) (· ≃ ·) (· ≃ ·)
+    := by
+  apply AA.CancellativeOn.mk
+  intro x y₁ y₂ (_ : x ≄ 0) (_ : x * y₁ ≃ x * y₂)
+  show y₁ ≃ y₂
+  have : Positive x := Signed.positive_defn.mpr ‹x ≄ 0›
+  have notTwoOfThree := (trichotomy (x * y₁) (x * y₂)).atMostOne
+  match (trichotomy y₁ y₂).atLeastOne with
+  | AA.OneOfThree.first (_ : y₁ < y₂) =>
+    have : x * y₁ < x * y₂ := AA.substRC ‹Positive x› ‹y₁ < y₂›
+    have twoOfThree :=
+      AA.TwoOfThree.oneAndTwo
+        (γ := x * y₁ > x * y₂) ‹x * y₁ < x * y₂› ‹x * y₁ ≃ x * y₂›
+    exact absurd twoOfThree notTwoOfThree
+  | AA.OneOfThree.second (_ : y₁ ≃ y₂) =>
+    exact ‹y₁ ≃ y₂›
+  | AA.OneOfThree.third (_ : y₁ > y₂) =>
+    have : y₂ < y₁ := ‹y₁ > y₂›
+    have : x * y₂ < x * y₁ := AA.substRC ‹Positive x› ‹y₂ < y₁›
+    have twoOfThree :=
+      AA.TwoOfThree.twoAndThree
+        (α := x * y₁ < x * y₂) ‹x * y₁ ≃ x * y₂› ‹x * y₂ < x * y₁›
+    exact absurd twoOfThree notTwoOfThree
 
-attribute [instance] Multiplication.Derived.mul_absorbing
-attribute [instance] Multiplication.Derived.mul_associative
-attribute [instance] Multiplication.Derived.mul_cancellative
-attribute [instance] Multiplication.Derived.mul_commutative
-attribute [instance] Multiplication.Derived.mul_distributive
-attribute [instance] Multiplication.Derived.mul_identity
-attribute [instance] Multiplication.Derived.mul_substitutive_eq
-attribute [instance] Multiplication.Derived.mul_substitutive_lt
+instance mul_cancellative
+    : AA.Cancellative (α := ℕ) (· * ·) (· ≄ 0) (· ≃ ·) (· ≃ ·)
+    := {
+  cancellativeL := mul_cancelL
+  cancellativeR := AA.cancelR_from_cancelL mul_cancelL
+}
 
-namespace Multiplication
-export Multiplication.Base (mulOp step_mul zero_mul)
-export Multiplication.Derived (
-  mul_associative mul_cancellative mul_commutative mul_distributive
-  mul_positive mul_split_zero mul_step mul_substitutive_eq mul_substitutive_lt
-)
-end Multiplication
+/--
+The natural number `1` is a left multiplicative identity element.
+
+**Property intuition**: A sum of a single instance of a number should be equal
+to that number.
+
+**Proof intuition**: Expand the definition of multiplication into addition to
+see that multiplying by one is the same as adding zero.
+-/
+theorem mul_identL {n : ℕ} : 1 * n ≃ n := calc
+  1 * n      ≃ _ := AA.substL Literals.literal_step
+  step 0 * n ≃ _ := step_mul
+  0 * n + n  ≃ _ := AA.substL zero_mul
+  0 + n      ≃ _ := AA.identL
+  n          ≃ _ := Rel.refl
+
+def mul_identityL : AA.IdentityOn Hand.L (α := ℕ) 1 (· * ·) := {
+  ident := mul_identL
+}
+
+instance mul_identity : AA.Identity (α := ℕ) 1 (· * ·) := {
+  identityL := mul_identityL
+  identityR := AA.identityR_from_identityL mul_identityL
+}
 
 end Lean4Axiomatic.Natural
