git/cruhland/lean4-axiomatic/Lean4Axiomatic/Natural/Order.lean
@@ -1,12 +1,16 @@
 import Lean4Axiomatic.Natural.Addition
 import Lean4Axiomatic.Natural.Sign
 
+/-!
+# Natural number ordering
+-/
+
 namespace Lean4Axiomatic.Natural
 
 open Signed (Positive)
 
 /-!
-# Definition and properties of natural number order
+## Axioms
 -/
 
 /--
@@ -14,7 +18,7 @@ Definition of the _less than or equal to_ and _less than_ relations.
 
 All other properties of ordering on natural numbers can be derived from this.
 -/
-class Order.Base (ℕ : Type) [Core ℕ] [Addition ℕ] :=
+class Order (ℕ : Type) [Core ℕ] [Addition ℕ] :=
   /-- Definition of and syntax for the _less than or equal to_ relation. -/
   leOp : LE ℕ
 
@@ -36,122 +40,610 @@ class Order.Base (ℕ : Type) [Core ℕ] [Addition ℕ] :=
   lt_defn {n m : ℕ} : n < m ↔ n ≤ m ∧ n ≄ m
 
 -- Higher priority than the stdlib definitions
-attribute [instance default+1] Order.Base.leOp
-attribute [instance default+1] Order.Base.ltOp
+attribute [instance default+1] Order.leOp
+attribute [instance default+1] Order.ltOp
 
-/-- Properties that follow from those provided in `Order.Base`. -/
-class Order.Derived
-    (ℕ : Type) [Core ℕ] [Addition ℕ] [Sign ℕ]
-    extends Order.Base ℕ
-    :=
-  /--
-  The _less than or equal to_ relation is preserved when both sides are
-  incremented.
-  -/
-  le_substitutive_step : AA.Substitutive₁ (α := ℕ) step (· ≤ ·) (· ≤ ·)
+export Order (le_defn leOp lt_defn ltOp)
 
-  /--
-  The _less than or equal to_ relation is preserved when both sides are
-  decremented.
-  -/
-  le_injective_step : AA.Injective (α := ℕ) step (· ≤ ·) (· ≤ ·)
+/-!
+## Derived properties
+-/
 
-  /--
-  Equal natural numbers can be substituted on either side of
-  _less than or equal to_.
-  -/
-  le_substitutive_eqv : AA.Substitutive₂ (α := ℕ) (· ≤ ·) AA.tc (· ≃ ·) (· → ·)
+variable {ℕ : Type}
+variable [Core ℕ]
+variable [Axioms ℕ]
+variable [Addition ℕ]
+variable [Sign ℕ]
+variable [Order ℕ]
 
-  /-- All natural numbers are _less than or equal to_ themselves. -/
-  le_reflexive : Relation.Reflexive (α := ℕ) (· ≤ ·)
+/--
+The _less than or equal to_ relation is preserved when both sides are
+incremented.
+-/
+theorem le_subst_step {n₁ n₂ : ℕ} : n₁ ≤ n₂ → step n₁ ≤ step n₂ := by
+  intro (_ : n₁ ≤ n₂)
+  show step n₁ ≤ step n₂
+  have ⟨d, (_ : n₁ + d ≃ n₂)⟩ := le_defn.mp ‹n₁ ≤ n₂›
+  apply le_defn.mpr
+  exists d
+  show step n₁ + d ≃ step n₂
+  calc
+    step n₁ + d   ≃ _ := step_add
+    step (n₁ + d) ≃ _ := AA.subst₁ ‹n₁ + d ≃ n₂›
+    step n₂       ≃ _ := Rel.refl
 
-  /--
-  The _less than or equal to_ relation can be extended through intermediate
-  values.
-  -/
-  le_transitive : Relation.Transitive (α := ℕ) (· ≤ ·)
+instance le_substitutive_step
+    : AA.Substitutive₁ (α := ℕ) step (· ≤ ·) (· ≤ ·)
+    := {
+  subst₁ := le_subst_step
+}
 
-  /-- Two natural numbers `n` and `m` are equal if `n ≤ m` and `m ≤ n`. -/
-  le_antisymm {n m : ℕ} : n ≤ m → m ≤ n → n ≃ m
+/--
+The _less than or equal to_ relation is preserved when both sides are
+decremented.
+-/
+theorem le_inject_step {n₁ n₂ : ℕ} : step n₁ ≤ step n₂ → n₁ ≤ n₂ := by
+  intro (_ : step n₁ ≤ step n₂)
+  show n₁ ≤ n₂
+  have ⟨d, (_ : step n₁ + d ≃ step n₂)⟩ := le_defn.mp ‹step n₁ ≤ step n₂›
+  apply le_defn.mpr
+  exists d
+  show n₁ + d ≃ n₂
+  have : step (n₁ + d) ≃ step n₂ := calc
+    step (n₁ + d) ≃ _ := Rel.symm step_add
+    step n₁ + d   ≃ _ := ‹step n₁ + d ≃ step n₂›
+    step n₂       ≃ _ := Rel.refl
+  exact AA.inject ‹step (n₁ + d) ≃ step n₂›
 
-  /--
-  The _less than or equal to_ relation is preserved when the same value is
-  added to both sides.
-  -/
-  le_substitutive_add : AA.Substitutive₂ (α := ℕ) (· + ·) AA.tc (· ≤ ·) (· ≤ ·)
+instance le_injective_step : AA.Injective (α := ℕ) step (· ≤ ·) (· ≤ ·) := {
+  inject := le_inject_step
+}
 
-  /--
-  The _less than or equal to_ relation is preserved when the same value is
-  removed from an addition on both sides.
-  -/
-  le_cancellative_add : AA.Cancellative (α := ℕ) (· + ·) AA.tc (· ≤ ·) (· ≤ ·)
+/--
+Equal natural numbers can be substituted on the left side of
+_less than or equal to_.
+-/
+theorem le_subst_eqv {n₁ n₂ m : ℕ} : n₁ ≃ n₂ → n₁ ≤ m → n₂ ≤ m := by
+  intro (_ : n₁ ≃ n₂) (_ : n₁ ≤ m)
+  show n₂ ≤ m
+  have ⟨d, (_ : n₁ + d ≃ m)⟩ := le_defn.mp ‹n₁ ≤ m›
+  apply le_defn.mpr
+  exists d
+  show n₂ + d ≃ m
+  calc
+    n₂ + d ≃ _ := Rel.symm (AA.substL ‹n₁ ≃ n₂›)
+    n₁ + d ≃ _ := ‹n₁ + d ≃ m›
+    m      ≃ _ := Rel.refl
 
-  /-- Weakens equality to _less than or equal to_. -/
-  le_from_eqv {n m : ℕ} : n ≃ m → n ≤ m
+def le_substL_eqv
+    : AA.SubstitutiveOn Hand.L (α := ℕ) (· ≤ ·) AA.tc (· ≃ ·) (· → ·)
+    := {
+  subst₂ := λ (_ : True) => le_subst_eqv
+}
 
-  /-- Weakens _less than_ to _less than or equal to_. -/
-  le_from_lt {n m : ℕ} : n < m → n ≤ m
+/--
+Equal natural numbers can be substituted on the right side of
+_less than or equal to_.
+-/
+theorem le_eqv_subst {n m₁ m₂ : ℕ} : m₁ ≃ m₂ → n ≤ m₁ → n ≤ m₂ := by
+  intro (_ : m₁ ≃ m₂) (_ : n ≤ m₁)
+  show n ≤ m₂
+  have ⟨d, (_ : n + d ≃ m₁)⟩ := le_defn.mp ‹n ≤ m₁›
+  apply le_defn.mpr
+  exists d
+  show n + d ≃ m₂
+  exact Rel.trans ‹n + d ≃ m₁› ‹m₁ ≃ m₂›
 
-  /--
-  As the name implies, if _less than or equal to_ holds between two natural
-  numbers, then either _less than_ holds between them as well, or the numbers
-  are equal.
-  -/
-  le_split {n m : ℕ} : n ≤ m → n < m ∨ n ≃ m
+def le_substR_eqv
+    : AA.SubstitutiveOn Hand.R (α := ℕ) (· ≤ ·) AA.tc (· ≃ ·) (· → ·)
+    := {
+  subst₂ := λ (_ : True) => le_eqv_subst
+}
 
-  /--
-  Equal natural numbers can be substituted on either side of _less than_.
-  -/
-  lt_substitutive_eqv : AA.Substitutive₂ (α := ℕ) (· < ·) AA.tc (· ≃ ·) (· → ·)
+instance le_substitutive_eqv
+    : AA.Substitutive₂ (α := ℕ) (· ≤ ·) AA.tc (· ≃ ·) (· → ·)
+    := {
+  substitutiveL := le_substL_eqv
+  substitutiveR := le_substR_eqv
+}
 
-  /-- The _less than_ relation can be extended through intermediate values. -/
-  lt_transitive : Relation.Transitive (α := ℕ) (· < ·)
+/-- All natural numbers are _less than or equal to_ themselves. -/
+theorem le_refl {n : ℕ} : n ≤ n := by
+  apply le_defn.mpr
+  exists (0 : ℕ)
+  show n + 0 ≃ n
+  exact add_zero
 
-  /-- No natural number is less than zero. -/
-  lt_zero {n : ℕ} : n ≮ 0
+instance le_reflexive : Relation.Reflexive (α := ℕ) (· ≤ ·) := {
+  refl := le_refl
+}
 
-  /-- A natural number is positive iff it's greater than zero. -/
-  lt_zero_pos {n : ℕ} : Positive n ↔ n > 0
+theorem le_step_split {n m : ℕ} : n ≤ step m → n ≤ m ∨ n ≃ step m := by
+  intro (_ : n ≤ step m)
+  show n ≤ m ∨ n ≃ step m
+  have ⟨d, (_ : n + d ≃ step m)⟩ := le_defn.mp ‹n ≤ step m›
+  let motive := λ x => d ≃ x → n ≤ m ∨ n ≃ step m
+  apply (cases_on (motive := motive) d · · Rel.refl)
+  · intro (_ : d ≃ 0)
+    apply Or.inr
+    show n ≃ step m
+    calc
+      n      ≃ _ := Rel.symm add_zero
+      n + 0  ≃ _ := AA.substR (Rel.symm ‹d ≃ 0›)
+      n + d  ≃ _ := ‹n + d ≃ step m›
+      step m ≃ _ := Rel.refl
+  · intro e (_ : d ≃ step e)
+    apply Or.inl
+    show n ≤ m
+    apply le_defn.mpr
+    exists e
+    show n + e ≃ m
+    apply AA.inject (β := ℕ) (rβ := (· ≃ ·))
+    show step (n + e) ≃ step m
+    calc
+      step (n + e) ≃ _ := Rel.symm add_step
+      n + step e   ≃ _ := AA.substR (Rel.symm ‹d ≃ step e›)
+      n + d        ≃ _ := ‹n + d ≃ step m›
+      step m       ≃ _ := Rel.refl
 
-  /-- A natural number is always less than its successor. -/
-  lt_step {n : ℕ} : n < step n
+theorem le_step {n m : ℕ} : n ≤ m → n ≤ step m := by
+  intro (_ : n ≤ m)
+  show n ≤ step m
+  have ⟨d, (_ : n + d ≃ m)⟩ := le_defn.mp ‹n ≤ m›
+  apply le_defn.mpr
+  exists step d
+  show n + step d ≃ step m
+  calc
+    n + step d   ≃ _ := add_step
+    step (n + d) ≃ _ := AA.subst₁ ‹n + d ≃ m›
+    step m       ≃ _ := Rel.refl
 
-  /--
-  A useful way to convert between _less than_ and _less than or equal to_ while
-  keeping the larger number fixed.
-  -/
-  lt_step_le {n m : ℕ} : n < m ↔ step n ≤ m
+/--
+The _less than or equal to_ relation can be extended through intermediate
+values.
+-/
+theorem le_trans {n m k : ℕ} : n ≤ m → m ≤ k → n ≤ k := by
+  intro (_ : n ≤ m)
+  have ⟨d, (_ : n + d ≃ m)⟩ := le_defn.mp ‹n ≤ m›
+  apply ind_on (motive := λ k => m ≤ k → n ≤ k) k
+  case zero =>
+    intro (_ : m ≤ 0)
+    have ⟨e, (_ : m + e ≃ 0)⟩ := le_defn.mp ‹m ≤ 0›
+    show n ≤ 0
+    apply le_defn.mpr
+    exists d + e
+    show n + (d + e) ≃ 0
+    calc
+      n + (d + e) ≃ _ := Rel.symm AA.assoc
+      (n + d) + e ≃ _ := AA.substL ‹n + d ≃ m›
+      m + e       ≃ _ := ‹m + e ≃ 0›
+      0           ≃ _ := Rel.refl
+  case step =>
+    intro k (ih : m ≤ k → n ≤ k) (_ : m ≤ step k)
+    show n ≤ step k
+    match le_step_split ‹m ≤ step k› with
+    | Or.inl (_ : m ≤ k) =>
+      exact le_step (ih ‹m ≤ k›)
+    | Or.inr (_ : m ≃ step k) =>
+      exact AA.substRFn ‹m ≃ step k› ‹n ≤ m›
 
-  /--
-  The _less than_ relation between two natural numbers `n` and `m` is
-  equivalent to there being a positive natural number -- the _difference_
-  between `n` and `m` -- that, when added to `n`, results in `m`.
-  -/
-  lt_defn_add {n m : ℕ} : n < m ↔ ∃ k, Positive k ∧ m ≃ n + k
+instance le_transitive : Relation.Transitive (α := ℕ) (· ≤ ·) := {
+  trans := le_trans
+}
 
-  /--
-  Useful result when needing to decrement the larger number in a _less than_
-  relation.
-  -/
-  lt_split {n m : ℕ} : n < step m → n < m ∨ n ≃ m
+/--
+The _less than or equal to_ relation is preserved when the same value is
+added on the left to both sides.
+-/
+theorem le_subst_add {n₁ n₂ m : ℕ} : n₁ ≤ n₂ → n₁ + m ≤ n₂ + m := by
+  intro (_ : n₁ ≤ n₂)
+  show n₁ + m ≤ n₂ + m
+  have ⟨d, (_ : n₁ + d ≃ n₂)⟩ := le_defn.mp ‹n₁ ≤ n₂›
+  apply le_defn.mpr
+  exists d
+  show (n₁ + m) + d ≃ n₂ + m
+  calc
+    (n₁ + m) + d ≃ _ := AA.assoc
+    n₁ + (m + d) ≃ _ := AA.substR AA.comm
+    n₁ + (d + m) ≃ _ := Rel.symm AA.assoc
+    (n₁ + d) + m ≃ _ := AA.substL ‹n₁ + d ≃ n₂›
+    n₂ + m       ≃ _ := Rel.refl
 
-  /--
-  Very general property about ordering which often simplifies proofs that would
-  otherwise have had to use induction.
-  -/
-  trichotomy (n m : ℕ) : AA.ExactlyOneOfThree (n < m) (n ≃ m) (n > m)
+def le_substL_add
+    : AA.SubstitutiveOn Hand.L (α := ℕ) (· + ·) AA.tc (· ≤ ·) (· ≤ ·)
+    := {
+  subst₂ := λ (_ : True) => le_subst_add
+}
 
-attribute [instance] Order.Derived.le_substitutive_eqv
-attribute [instance] Order.Derived.lt_substitutive_eqv
-attribute [instance] Order.Derived.lt_transitive
+instance le_substitutive_add
+    : AA.Substitutive₂ (α := ℕ) (· + ·) AA.tc (· ≤ ·) (· ≤ ·)
+    := {
+  substitutiveL := le_substL_add
+  substitutiveR := AA.substR_from_substL_swap (rS := (· ≃ ·)) le_substL_add
+}
 
-namespace Order
-export Order.Base (le_defn leOp lt_defn ltOp)
-export Order.Derived (
-  le_antisymm le_reflexive le_split le_transitive
-  lt_defn_add lt_split lt_step lt_step_le lt_transitive lt_zero lt_zero_pos
-  trichotomy
-)
-end Order
+/--
+The _less than or equal to_ relation is preserved when the same value is
+removed from the left side of an addition on both sides of an equivalence.
+-/
+theorem le_cancel_add {n m₁ m₂ : ℕ} : n + m₁ ≤ n + m₂ → m₁ ≤ m₂ := by
+  intro (_ : n + m₁ ≤ n + m₂)
+  show m₁ ≤ m₂
+  have ⟨d, (_ : (n + m₁) + d ≃ n + m₂)⟩ := le_defn.mp ‹n + m₁ ≤ n + m₂›
+  apply le_defn.mpr
+  exists d
+  show m₁ + d ≃ m₂
+  have : n + (m₁ + d) ≃ n + m₂ := calc
+    n + (m₁ + d) ≃ _ := Rel.symm AA.assoc
+    (n + m₁) + d ≃ _ := ‹(n + m₁) + d ≃ n + m₂›
+    n + m₂       ≃ _ := Rel.refl
+  exact AA.cancelL ‹n + (m₁ + d) ≃ n + m₂›
+
+def le_cancelL_add
+    : AA.CancellativeOn Hand.L (α := ℕ) (· + ·) AA.tc (· ≤ ·) (· ≤ ·)
+    := {
+  cancel := λ (_ : True) => le_cancel_add
+}
+
+instance le_cancellative_add
+    : AA.Cancellative (α := ℕ) (· + ·) AA.tc (· ≤ ·) (· ≤ ·) := {
+  cancellativeL := le_cancelL_add
+  cancellativeR := AA.cancelR_from_cancelL le_cancelL_add
+}
+
+/-- Two natural numbers `n` and `m` are equal if `n ≤ m` and `m ≤ n`. -/
+theorem le_antisymm {n m : ℕ} : n ≤ m → m ≤ n → n ≃ m := by
+  intro (_ : n ≤ m) (_ : m ≤ n)
+  show n ≃ m
+  have ⟨d₁, (_ : n + d₁ ≃ m)⟩ := le_defn.mp ‹n ≤ m›
+  have ⟨d₂, (_ : m + d₂ ≃ n)⟩ := le_defn.mp ‹m ≤ n›
+  have : n + (d₁ + d₂) ≃ n + 0 := calc
+    n + (d₁ + d₂) ≃ _ := Rel.symm AA.assoc
+    (n + d₁) + d₂ ≃ _ := AA.substL ‹n + d₁ ≃ m›
+    m + d₂        ≃ _ := ‹m + d₂ ≃ n›
+    n             ≃ _ := Rel.symm add_zero
+    n + 0         ≃ _ := Rel.refl
+  have : d₁ + d₂ ≃ 0 := AA.cancelL ‹n + (d₁ + d₂) ≃ n + 0›
+  have ⟨(_ : d₁ ≃ 0), _⟩ := zero_sum_split ‹d₁ + d₂ ≃ 0›
+  calc
+    n      ≃ _ := Rel.symm add_zero
+    n + 0  ≃ _ := AA.substR (Rel.symm ‹d₁ ≃ 0›)
+    n + d₁ ≃ _ := ‹n + d₁ ≃ m›
+    m      ≃ _ := Rel.refl
+
+/--
+Equivalent natural numbers can be substituted on the left side of _less than_.
+-/
+theorem lt_subst_eqv {n₁ n₂ m : ℕ} : n₁ ≃ n₂ → n₁ < m → n₂ < m := by
+  intro (_ : n₁ ≃ n₂) (_ : n₁ < m)
+  show n₂ < m
+  have ⟨(_ : n₁ ≤ m), (_ : n₁ ≄ m)⟩ := lt_defn.mp ‹n₁ < m›
+  have : n₂ ≤ m := AA.substLFn ‹n₁ ≃ n₂› ‹n₁ ≤ m›
+  have : n₂ ≄ m := AA.substLFn (f := (· ≄ ·)) ‹n₁ ≃ n₂› ‹n₁ ≄ m›
+  apply lt_defn.mpr
+  exact ⟨‹n₂ ≤ m›, ‹n₂ ≄ m›⟩
+
+def lt_substL_eqv
+    : AA.SubstitutiveOn Hand.L (α := ℕ) (· < ·) AA.tc (· ≃ ·) (· → ·)
+    := {
+  subst₂ := λ (_ : True) => lt_subst_eqv
+}
+
+/--
+Equivalent natural numbers can be substituted on the right side of _less than_.
+-/
+theorem lt_eqv_subst {n₁ n₂ m : ℕ} : n₁ ≃ n₂ → m < n₁ → m < n₂ := by
+  intro (_ : n₁ ≃ n₂) (_ : m < n₁)
+  show m < n₂
+  have ⟨(_ : m ≤ n₁), (_ : m ≄ n₁)⟩ := lt_defn.mp ‹m < n₁›
+  have : m ≤ n₂ := AA.substRFn ‹n₁ ≃ n₂› ‹m ≤ n₁›
+  have : m ≄ n₂ := AA.substRFn (f := (· ≄ ·)) ‹n₁ ≃ n₂› ‹m ≄ n₁›
+  apply lt_defn.mpr
+  exact ⟨‹m ≤ n₂›, ‹m ≄ n₂›⟩
+
+def lt_substR_eqv
+    : AA.SubstitutiveOn Hand.R (α := ℕ) (· < ·) AA.tc (· ≃ ·) (· → ·)
+    := {
+  subst₂ := λ (_ : True) => lt_eqv_subst
+}
+
+instance lt_substitutive_eqv
+    : AA.Substitutive₂ (α := ℕ) (· < ·) AA.tc (· ≃ ·) (· → ·)
+    := {
+  substitutiveL := lt_substL_eqv
+  substitutiveR := lt_substR_eqv
+}
+
+/-- A natural number is always less than its successor. -/
+theorem lt_step {n : ℕ} : n < step n := by
+  show n < step n
+  apply lt_defn.mpr
+  apply And.intro
+  · show n ≤ step n
+    apply le_defn.mpr
+    exists (1 : ℕ)
+    show n + 1 ≃ step n
+    exact add_one_step
+  · show n ≄ step n
+    exact Rel.symm step_neq
+
+/--
+A useful way to convert between _less than_ and _less than or equal to_ while
+keeping the larger number fixed.
+-/
+theorem lt_step_le {n m : ℕ} : n < m ↔ step n ≤ m := by
+  apply Iff.intro
+  · intro (_ : n < m)
+    show step n ≤ m
+    have ⟨(_ : n ≤ m), (_ : n ≄ m)⟩ := lt_defn.mp ‹n < m›
+    have ⟨d, (_ : n + d ≃ m)⟩ := le_defn.mp ‹n ≤ m›
+    have : d ≄ 0 := by
+      intro (_ : d ≃ 0)
+      show False
+      apply ‹n ≄ m›
+      show n ≃ m
+      calc
+        n     ≃ _ := Rel.symm add_zero
+        n + 0 ≃ _ := AA.substR (Rel.symm ‹d ≃ 0›)
+        n + d ≃ _ := ‹n + d ≃ m›
+        m     ≃ _ := Rel.refl
+    have : Positive d := Signed.positive_defn.mpr ‹d ≄ 0›
+    have ⟨d', (_ : step d' ≃ d)⟩ := positive_step ‹Positive d›
+    show step n ≤ m
+    apply le_defn.mpr
+    exists d'
+    show step n + d' ≃ m
+    calc
+      step n + d'   ≃ _ := step_add
+      step (n + d') ≃ _ := Rel.symm add_step
+      n + step d'   ≃ _ := AA.substR ‹step d' ≃ d›
+      n + d         ≃ _ := ‹n + d ≃ m›
+      m             ≃ _ := Rel.refl
+  · intro (_ : step n ≤ m)
+    show n < m
+    have ⟨d, (_ : step n + d ≃ m)⟩ := le_defn.mp ‹step n ≤ m›
+    have : n + step d ≃ m := calc
+      n + step d   ≃ _ := add_step
+      step (n + d) ≃ _ := Rel.symm step_add
+      step n + d   ≃ _ := ‹step n + d ≃ m›
+      m            ≃ _ := Rel.refl
+    have : ∃ d, n + d ≃ m := ⟨step d, ‹n + step d ≃ m›⟩
+    have : n ≤ m := le_defn.mpr ‹∃ d, n + d ≃ m›
+    have : n ≄ m := by
+      intro (_ : n ≃ m)
+      show False
+      have : n + step d ≃ n + 0 := calc
+        n + step d ≃ _ := ‹n + step d ≃ m›
+        m          ≃ _ := Rel.symm ‹n ≃ m›
+        n          ≃ _ := Rel.symm add_zero
+        n + 0      ≃ _ := Rel.refl
+      have : step d ≃ 0 := AA.cancelL ‹n + step d ≃ n + 0›
+      exact absurd this Axioms.step_neq_zero
+    show n < m
+    apply lt_defn.mpr
+    exact ⟨‹n ≤ m›, ‹n ≄ m›⟩
+
+/--
+The _less than_ relation between two natural numbers `n` and `m` is
+equivalent to there being a positive natural number -- the _difference_
+between `n` and `m` -- that, when added to `n`, results in `m`.
+
+**Intuition**: This is already quite intuitive, as it's clear that for one
+number to be less than another, there must be a nonzero gap between them.
+-/
+theorem lt_defn_add {n m : ℕ} : n < m ↔ ∃ k, Positive k ∧ m ≃ n + k := by
+  apply Iff.intro
+  · intro (_ : n < m)
+    show ∃ k, Positive k ∧ m ≃ n + k
+    have : step n ≤ m := lt_step_le.mp ‹n < m›
+    have ⟨k, (_ : step n + k ≃ m)⟩ := le_defn.mp ‹step n ≤ m›
+    exists step k
+    apply And.intro
+    · show Positive (step k)
+      apply Signed.positive_defn.mpr
+      show step k ≄ 0
+      exact Axioms.step_neq_zero
+    · show m ≃ n + step k
+      calc
+        m            ≃ _ := Rel.symm ‹step n + k ≃ m›
+        step n + k   ≃ _ := step_add
+        step (n + k) ≃ _ := Rel.symm add_step
+        n + step k   ≃ _ := Rel.refl
+  · intro ⟨k, (_ : Positive k), (_ : m ≃ n + k)⟩
+    show n < m
+    apply lt_step_le.mpr
+    show step n ≤ m
+    apply le_defn.mpr
+    show ∃ k, step n + k ≃ m
+    have ⟨k', (_ : step k' ≃ k)⟩ := positive_step ‹Positive k›
+    exists k'
+    show step n + k' ≃ m
+    calc
+      step n + k'   ≃ _ := step_add
+      step (n + k') ≃ _ := Rel.symm add_step
+      n + step k'   ≃ _ := AA.substR ‹step k' ≃ k›
+      n + k         ≃ _ := Rel.symm ‹m ≃ n + k›
+      m             ≃ _ := Rel.refl
+
+/-- No natural number is less than zero. -/
+theorem lt_zero {n : ℕ} : n ≮ 0 := by
+  intro (_ : n < 0)
+  show False
+  have : step n ≤ 0 := lt_step_le.mp ‹n < 0›
+  have ⟨d, (_ : step n + d ≃ 0)⟩ := le_defn.mp ‹step n ≤ 0›
+  have : step (n + d) ≃ 0 := calc
+    step (n + d) ≃ _ := Rel.symm step_add
+    step n + d   ≃ _ := ‹step n + d ≃ 0›
+    0            ≃ _ := Rel.refl
+  exact absurd ‹step (n + d) ≃ 0› Axioms.step_neq_zero
+
+/--
+A natural number is positive iff it's greater than zero.
+
+**Proof intuition**: The _less than_ relation can be defined in terms of a
+positive difference between its two arguments. If the left argument is zero,
+then the right argument must be positive.
+-/
+theorem lt_zero_pos {n : ℕ} : Positive n ↔ n > 0 := by
+  apply Iff.intro
+  · intro (_ : Positive n)
+    show 0 < n
+    apply lt_defn_add.mpr
+    show ∃ k, Positive k ∧ n ≃ 0 + k
+    exists n
+    apply And.intro
+    · show Positive n
+      exact ‹Positive n›
+    · show n ≃ 0 + n
+      exact Rel.symm zero_add
+  · intro (_ : 0 < n)
+    show Positive n
+    have ⟨k, ⟨(_ : Positive k), (_ : n ≃ 0 + k)⟩⟩ := lt_defn_add.mp ‹0 < n›
+    have : k ≃ n := Rel.symm (Rel.trans ‹n ≃ 0 + k› zero_add)
+    exact AA.subst₁ (f := Positive) (rβ := (· → ·)) ‹k ≃ n› ‹Positive k›
+
+/-- Weakens equivalence to _less than or equal to_. -/
+theorem le_from_eqv {n m : ℕ} : n ≃ m → n ≤ m := by
+  intro (_ : n ≃ m)
+  show n ≤ m
+  have : n ≤ n := Rel.refl
+  exact AA.substRFn ‹n ≃ m› ‹n ≤ n›
+
+/-- Weakens _less than_ to _less than or equal to_. -/
+theorem le_from_lt {n m : ℕ} : n < m → n ≤ m := by
+  intro (_ : n < m)
+  show n ≤ m
+  have ⟨(_ : n ≤ m), _⟩ := lt_defn.mp ‹n < m›
+  exact ‹n ≤ m›
+
+/--
+As the name implies, if _less than or equal to_ holds between two natural
+numbers, then either _less than_ holds between them as well, or the numbers are
+equivalent.
+-/
+theorem le_split {n m : ℕ} : n ≤ m → n < m ∨ n ≃ m := by
+  intro (_ : n ≤ m)
+  show n < m ∨ n ≃ m
+  have ⟨d, (h : n + d ≃ m)⟩ := le_defn.mp ‹n ≤ m›
+  revert h
+  apply cases_on (motive := λ d => n + d ≃ m → n < m ∨ n ≃ m) d
+  case zero =>
+    intro (_ : n + 0 ≃ m)
+    apply Or.inr
+    show n ≃ m
+    calc
+      n     ≃ _ := Rel.symm add_zero
+      n + 0 ≃ _ := ‹n + 0 ≃ m›
+      m     ≃ _ := Rel.refl
+  case step =>
+    intro d (_ : n + step d ≃ m)
+    apply Or.inl
+    show n < m
+    apply lt_step_le.mpr
+    show step n ≤ m
+    apply le_defn.mpr
+    exists d
+    show step n + d ≃ m
+    calc
+      step n + d   ≃ _ := step_add
+      step (n + d) ≃ _ := Rel.symm add_step
+      n + step d   ≃ _ := ‹n + step d ≃ m›
+      m            ≃ _ := Rel.refl
+
+/--
+Useful result when needing to decrement the larger number in a _less than_
+relation.
+-/
+theorem lt_split {n m : ℕ} : n < step m → n < m ∨ n ≃ m := by
+  intro (_ : n < step m)
+  show n < m ∨ n ≃ m
+  have : step n ≤ step m := lt_step_le.mp ‹n < step m›
+  have : n ≤ m := AA.inject ‹step n ≤ step m›
+  exact le_split ‹n ≤ m›
+
+/-- The _less than_ relation can be extended through intermediate values. -/
+theorem lt_trans {n m k : ℕ} : n < m → m < k → n < k := by
+  intro (_ : n < m) (_ : m < k)
+  show n < k
+  apply lt_step_le.mpr
+  show step n ≤ k
+  calc
+    step n ≤ _ := lt_step_le.mp ‹n < m›
+    m      ≤ _ := le_from_lt lt_step
+    step m ≤ _ := lt_step_le.mp ‹m < k›
+    k      ≤ _ := Rel.refl
+
+instance lt_transitive : Relation.Transitive (α := ℕ) (· < ·) := {
+  trans := lt_trans
+}
+
+/--
+Very general property about ordering which often simplifies proofs that would
+otherwise have had to use induction.
+-/
+theorem trichotomy (n m : ℕ)
+    : AA.ExactlyOneOfThree (n < m) (n ≃ m) (n > m) := by
+  constructor
+  case atLeastOne =>
+    let motive := λ n => AA.OneOfThree (n < m) (n ≃ m) (n > m)
+    apply ind_on (motive := motive) n
+    case zero =>
+      show AA.OneOfThree (0 < m) (0 ≃ m) (0 > m)
+      let motive := λ m : ℕ => AA.OneOfThree (0 < m) (0 ≃ m) (0 > m)
+      apply cases_on (motive := motive) m
+      case zero =>
+        apply AA.OneOfThree.second
+        show 0 ≃ 0
+        exact Rel.refl
+      case step =>
+        intro m
+        apply AA.OneOfThree.first
+        show 0 < step m
+        apply lt_defn.mpr
+        apply And.intro
+        · show 0 ≤ step m
+          apply le_defn.mpr
+          exists step m
+          exact zero_add
+        · show 0 ≄ step m
+          exact Rel.symm Axioms.step_neq_zero
+    case step =>
+      intro n (ih : AA.OneOfThree (n < m) (n ≃ m) (n > m))
+      show AA.OneOfThree (step n < m) (step n ≃ m) (step n > m)
+      match ih with
+      | AA.OneOfThree.first (_ : n < m) =>
+        have : step n ≤ m := lt_step_le.mp ‹n < m›
+        have : step n < m ∨ step n ≃ m := le_split ‹step n ≤ m›
+        match ‹step n < m ∨ step n ≃ m› with
+        | Or.inl (_ : step n < m) => exact AA.OneOfThree.first ‹step n < m›
+        | Or.inr (_ : step n ≃ m) => exact AA.OneOfThree.second ‹step n ≃ m›
+      | AA.OneOfThree.second (_ : n ≃ m) =>
+        have : m ≃ n := Rel.symm ‹n ≃ m›
+        have : m ≤ n := le_from_eqv ‹m ≃ n›
+        have : step m ≤ step n := AA.subst₁ ‹m ≤ n›
+        have : m < step n := lt_step_le.mpr ‹step m ≤ step n›
+        apply AA.OneOfThree.third
+        exact ‹m < step n›
+      | AA.OneOfThree.third (_ : n > m) =>
+        apply AA.OneOfThree.third
+        show m < step n
+        exact Rel.trans ‹m < n› lt_step
+  case atMostOne =>
+    show ¬ AA.TwoOfThree (n < m) (n ≃ m) (n > m)
+    intro
+    | AA.TwoOfThree.oneAndTwo (_ : n < m) (_ : n ≃ m) =>
+      show False
+      have ⟨_, (_ : n ≄ m)⟩ := lt_defn.mp ‹n < m›
+      exact absurd ‹n ≃ m› ‹n ≄ m›
+    | AA.TwoOfThree.oneAndThree (_ : n < m) (_ : n > m) =>
+      show False
+      have ⟨(_ : n ≤ m), (_ : n ≄ m)⟩ := lt_defn.mp ‹n < m›
+      have ⟨(_ : m ≤ n), _⟩ := lt_defn.mp ‹n > m›
+      have : n ≃ m := le_antisymm ‹n ≤ m› ‹m ≤ n›
+      exact absurd ‹n ≃ m› ‹n ≄ m›
+    | AA.TwoOfThree.twoAndThree (_ : n ≃ m) (_ : n > m) =>
+      show False
+      have ⟨_, (_ : m ≄ n)⟩ := lt_defn.mp ‹n > m›
+      exact absurd ‹n ≃ m› (Rel.symm ‹m ≄ n›)
 
 end Lean4Axiomatic.Natural
