git/cruhland/lean4-analysis/Lean4Analysis/Ch2.lean
@@ -13,13 +13,10 @@ namespace AnalysisI.Ch2
 
 namespace Impl
 
-export Natural.Default (order_base sign)
-export Natural.Derived (
-  multiplication_derived order_derived
-)
+export Natural.Default (order sign)
 export Natural.Impl.Nat (
-  addition axioms constructors core equality exponentiation_base
-  literals multiplication_base
+  addition axioms constructors core equality exponentiation literals
+  multiplication
 )
 
 end Impl
@@ -272,9 +269,9 @@ example {a : ℕ}
 -- _greater than or equal to_ `m`, and write `n ≥ m` or `m ≤ n`, iff we have
 -- `n ≃ m + a` for some natural number `a`.
 example : ℕ → ℕ → Prop :=
-  @GE.ge ℕ (Natural.leOp (self := Impl.order_base))
+  @GE.ge ℕ (Natural.leOp (self := Impl.order))
 example {n m : ℕ} : n ≥ m ↔ ∃ a : ℕ, n ≃ m + a := by
-  let le_defn := @Natural.le_defn (ℕ := ℕ) (self := Impl.order_base)
+  let le_defn := @Natural.le_defn (ℕ := ℕ) (self := Impl.order)
   apply Iff.intro
   · intro (_ : m ≤ n)
     show ∃ a, n ≃ m + a
@@ -287,9 +284,9 @@ example {n m : ℕ} : n ≥ m ↔ ∃ a : ℕ, n ≃ m + a := by
 -- We say that `n` is _strictly greater than_ `m`, and write `n > m` or
 -- `m < n`, iff `n ≥ m` and `n ≄ m`.
 example : ℕ → ℕ → Prop :=
-  @GT.gt ℕ (Natural.ltOp (self := Impl.order_base))
+  @GT.gt ℕ (Natural.ltOp (self := Impl.order))
 example {n m : ℕ} : n > m ↔ n ≥ m ∧ n ≄ m := by
-  let lt_defn := @Natural.lt_defn (ℕ := ℕ) (self := Impl.order_base)
+  let lt_defn := @Natural.lt_defn (ℕ := ℕ) (self := Impl.order)
   apply Iff.intro
   · intro (_ : n > m)
     show n ≥ m ∧ n ≄ m
@@ -315,19 +312,17 @@ example : 8 > 5 := by
     rfl
 
 -- Also note that `step n > n` for any `n`
-example {n : ℕ} : step n > n :=
-  Natural.lt_step (self := Impl.order_derived)
+example {n : ℕ} : step n > n := Natural.lt_step
 
 -- Exercise 2.2.3.
 -- Proposition 2.2.12 (Basic properties of order for natural numbers).
 -- Let `a`, `b`, `c` be natural numbers. Then
 -- (a) (Order is reflexive) `a ≥ a`.
-example {a : ℕ} : a ≥ a :=
-  Rel.refl (self := Natural.le_reflexive (self := Impl.order_derived))
+example {a : ℕ} : a ≥ a := Rel.refl (self := Natural.le_reflexive)
 
 -- (b) (Order is transitive) If `a ≥ b` and `b ≥ c`, then `a ≥ c`.
 example {a b c : ℕ} : a ≥ b → b ≥ c → a ≥ c :=
-  flip (Rel.trans (self := Natural.le_transitive (self := Impl.order_derived)))
+  flip (Rel.trans (self := Natural.le_transitive))
 
 -- (c) (Order is anti-symmetric) If `a ≥ b` and `b ≥ a`, then `a ≃ b`.
 example {a b : ℕ} : a ≥ b → b ≥ a → a ≃ b := flip Natural.le_antisymm
@@ -343,8 +338,7 @@ example {a b c : ℕ} : a ≥ b ↔ a + c ≥ b + c := by
     exact AA.cancelR ‹b + c ≤ a + c›
 
 -- (e) `a < b` if and only if `step a ≤ b`.
-example {a b : ℕ} : a < b ↔ step a ≤ b :=
-  Natural.lt_step_le (self := Impl.order_derived)
+example {a b : ℕ} : a < b ↔ step a ≤ b := Natural.lt_step_le
 
 -- (f) `a < b` if and only if `b ≃ a + d` for some _positive_ number `d`.
 example {a b : ℕ} : a < b ↔ ∃ d, Positive d ∧ b ≃ a + d := Natural.lt_defn_add
@@ -354,7 +348,7 @@ example {a b : ℕ} : a < b ↔ ∃ d, Positive d ∧ b ≃ a + d := Natural.lt_
 -- Let `a` and `b` be natural numbers. Then exactly one of the following
 -- statements is true: `a < b`, `a ≃ b`, or `a > b`.
 example {a b : ℕ} : AA.ExactlyOneOfThree (a < b) (a ≃ b) (a > b) :=
-  Natural.trichotomy (self := Impl.order_derived) a b
+  Natural.trichotomy a b
 
 -- Exercise 2.2.5.
 -- Proposition 2.2.14 (Strong principle of induction).
@@ -378,12 +372,12 @@ example
   case zero =>
     intro m' (_ : m₀ ≤ m') (_ : m' < 0)
     show P m'
-    exact absurd ‹m' < 0› (Natural.lt_zero (self := Impl.order_derived))
+    exact absurd ‹m' < 0› (Natural.lt_zero)
   case step =>
     intro m (ih : ∀ m', m₀ ≤ m' → m' < m → P m')
     intro m' (_ : m₀ ≤ m') (_ : m' < step m)
     show P m'
-    match Natural.lt_split (self := Impl.order_derived) ‹m' < step m› with
+    match Natural.lt_split ‹m' < step m› with
     | Or.inl (_ : m' < m) =>
       exact ih m' ‹m₀ ≤ m'› ‹m' < m›
     | Or.inr (_ : m' ≃ m) =>
@@ -405,7 +399,7 @@ example {P : ℕ → Prop} [AA.Substitutive₁ P (· ≃ ·) (· → ·)] {n : �
   case zero =>
     intro (_ : P 0) m (_ : m ≤ 0)
     show P m
-    match Natural.le_split (self := Impl.order_derived) ‹m ≤ 0› with
+    match Natural.le_split ‹m ≤ 0› with
     | Or.inl (_ : m < 0) =>
       exact absurd ‹m < 0› Natural.lt_zero
     | Or.inr (_ : m ≃ 0) =>
@@ -430,20 +424,16 @@ example {P : ℕ → Prop} [AA.Substitutive₁ P (· ≃ ·) (· → ·)] {n : �
 -- `n` to `m`. Then we can multiply `step n` to `m` by defining
 -- `step n * m := (n * m) + m`.
 example : ℕ → ℕ → ℕ :=
-  Mul.mul (self := Natural.mulOp (self := Impl.multiplication_base))
+  Mul.mul (self := Natural.mulOp (self := Impl.multiplication))
 
-example {m : ℕ} : 0 * m ≃ 0 :=
-  Natural.zero_mul (self := Impl.multiplication_base)
+example {m : ℕ} : 0 * m ≃ 0 := Natural.zero_mul (self := Impl.multiplication)
 
 example {n m : ℕ} : step n * m ≃ (n * m) + m :=
-  Natural.step_mul (self := Impl.multiplication_base)
-
--- [Shorter name for convenient reference below]
-abbrev mul_derived := Impl.multiplication_derived (ℕ := ℕ)
+  Natural.step_mul (self := Impl.multiplication)
 
 -- [Multiplication obeys left and right substitution]
 example : AA.Substitutive₂ (α := ℕ) (· * ·) AA.tc (· ≃ ·) (· ≃ ·) :=
-  Natural.mul_substitutive_eq (self := mul_derived)
+  Natural.mul_substitutive_eq
 
 -- Thus for instance `0 * m ≃ 0`,
 def ex_zero_mul {m : ℕ} : 0 * m ≃ 0 := Natural.zero_mul
@@ -471,26 +461,24 @@ def two_mul_sum {m : ℕ} : 2 * m ≃ m + m := calc
 -- Lemma 2.3.2 (Multiplication is commutative).
 -- Let `n`, `m` be natural numbers. Then `n * m ≃ m * n`.
 example {n m : ℕ} : n * m ≃ m * n := by
-  exact AA.comm (self := Natural.mul_commutative (self := mul_derived))
+  exact AA.comm (self := Natural.mul_commutative)
 
 -- Exercise 2.3.2.
 -- Lemma 2.3.3 (Positive natural numbers have no zero divisors).
 -- Let `n`, `m` be natural numbers. Then `n * m ≃ 0` if and only if at least
 -- one of `n`, `m` is equal to zero.
-example {n m : ℕ} : n * m ≃ 0 ↔ n ≃ 0 ∨ m ≃ 0 :=
-  Natural.mul_split_zero (self := mul_derived)
+example {n m : ℕ} : n * m ≃ 0 ↔ n ≃ 0 ∨ m ≃ 0 := Natural.mul_split_zero
 
 -- In particular, if `n` and `m` are both positive, then `n * m` is also
 -- positive.
 example {n m : ℕ} : Positive n → Positive m → Positive (n * m) :=
-  Natural.mul_positive (self := mul_derived)
+  Natural.mul_positive
 
 -- Proposition 2.3.4 (Distributive law).
 -- For any natural numbers `a`, `b`, `c`, we have `a * (b + c) ≃ a * b + a * c`
 -- and `(b + c) * a ≃ b * a + c * a`.
 example {a b c : ℕ} : a * (b + c) ≃ a * b + a * c :=
-  let mul_distributive := Natural.mul_distributive (self := mul_derived)
-  AA.distrib (self := mul_distributive.distributiveL)
+  AA.distrib (self := Natural.mul_distributive.distributiveL)
 
 example {a b c : ℕ} : (b + c) * a ≃ b * a + c * a := AA.distribR
 
@@ -498,7 +486,7 @@ example {a b c : ℕ} : (b + c) * a ≃ b * a + c * a := AA.distribR
 -- Proposition 2.3.5 (Multiplication is associative).
 -- For any natural numbers `a`, `b`, `c`, we have `(a * b) * c ≃ a * (b * c)`.
 example {a b c : ℕ} : (a * b) * c ≃ a * (b * c) :=
-  AA.assoc (self := Natural.mul_associative (self := mul_derived))
+  AA.assoc (self := Natural.mul_associative)
 
 -- Proposition 2.3.6 (Multiplication preserves order).
 -- If `a`, `b` are natural numbers such that `a < b`, and `c` is positive, then
@@ -506,8 +494,7 @@ example {a b c : ℕ} : (a * b) * c ≃ a * (b * c) :=
 example {a b c : ℕ} : a < b → Positive c → a * c < b * c := by
   intro (_ : a < b) (_ : Positive c)
   show a * c < b * c
-  let mul_substitutive_lt := Natural.mul_substitutive_lt (self := mul_derived)
-  let mul_substL_lt := mul_substitutive_lt.substitutiveL
+  let mul_substL_lt := (Natural.mul_substitutive_lt (ℕ := ℕ)).substitutiveL
   exact AA.substLC (self := mul_substL_lt) ‹Positive c› ‹a < b›
 
 -- Corollary 2.3.7 (Cancellation law).
@@ -516,8 +503,7 @@ example {a b c : ℕ} : a < b → Positive c → a * c < b * c := by
 example {a b c : ℕ} : a * c ≃ b * c → c ≄ 0 → a ≃ b := by
   intro (_ : a * c ≃ b * c) (_ : c ≄ 0)
   show a ≃ b
-  let mul_cancellative := Natural.mul_cancellative (self := mul_derived)
-  let mul_cancelR := mul_cancellative.cancellativeR
+  let mul_cancelR := (Natural.mul_cancellative (ℕ := ℕ)).cancellativeR
   exact AA.cancelRC (self := mul_cancelR) ‹c ≄ 0› ‹a * c ≃ b * c›
 
 -- Exercise 2.3.5
@@ -578,12 +564,11 @@ theorem euclidean_algorithm {n q : ℕ} : Positive q → Euclid n q := by
 
 -- Definition 2.3.11 (Exponentiation for natural numbers).
 example : ℕ → ℕ → ℕ :=
-  Pow.pow (self := Natural.powOp (self := Impl.exponentiation_base))
+  Pow.pow (self := Natural.powOp (self := Impl.exponentiation))
 
 -- Let `m` be a natural number. To raise `m` to the power `0`, we define
 -- `m ^ 0 := 1`;
-example {m : ℕ} : m ^ 0 ≃ 1 :=
-  Natural.pow_zero (self := Impl.exponentiation_base)
+example {m : ℕ} : m ^ 0 ≃ 1 := Natural.pow_zero (self := Impl.exponentiation)
 
 -- in particular, we define `0 ^ 0 := 1`.
 example : 0 ^ (0 : ℕ) ≃ 1 := Natural.pow_zero
@@ -591,7 +576,7 @@ example : 0 ^ (0 : ℕ) ≃ 1 := Natural.pow_zero
 -- Now suppose recursively that `m ^ n` has been defined for some natural
 -- number `n`, then we define `m ^ step n := m ^ n * m`.
 example {m n : ℕ} : m ^ step n ≃ m ^ n * m :=
-  Natural.pow_step (self := Impl.exponentiation_base)
+  Natural.pow_step (self := Impl.exponentiation)
 
 -- Examples 2.3.12.
 -- Thus for instance `x ^ 1 ≃ x ^ 0 * x ≃ 1 * x ≃ x`;
