git/cruhland/lean4-axiomatic/Lean4Axiomatic/Natural/Impl/Derived.lean
@@ -1,2 +1,0 @@
-import Lean4Axiomatic.Natural.Impl.Derived.Multiplication
-import Lean4Axiomatic.Natural.Impl.Derived.Order
